Abstract more theorems about fields and ordered rings.

fields.v
@@ -39,6 +39,7 @@ Section Field_theorems.
   Notation "a '^-1' " := (inv_F _ a) (at level 30, format "a '^-1'").
 
   Definition sub_F a b := a + (-b).
+  Definition inv_l := M4_F.
 
   Infix "-" := sub_F.
 
@@ -56,7 +57,6 @@ Section Field_theorems.
     auto.
   Qed.
 
-
   Add Field generic_field :
     (mk_field div_F
               (inv_F F)
@@ -68,6 +68,13 @@ Section Field_theorems.
   Definition ring_from_field :=
     mkRing _ 0 1 (add_F F) (mul_F F) (neg_F F) (A3_F F) (A1_F F) (A2_F F)
            (M3_F F) (M1_F F) (M2_F F) (D1_F F) (A4_F F).
+
+  Theorem inv_r : ∀ a, a ≠ 0 → a * a^-1 = 1.
+  Proof.
+    intros a H.
+    now field.
+  Qed.
+  Definition M4_R := inv_r.
 
   Theorem cancellation : ∀ a b, a * b = 0 → a = 0 ∨ b = 0.
   Proof.
@@ -81,5 +88,50 @@ Section Field_theorems.
 
   Definition integral_domain_from_field :=
     mkID ring_from_field cancellation (one_ne_0_F F).
+
+  Theorem inv_unique : ∀ a, (∀ b, a * b = 1 → b = a^-1).
+  Proof.
+    intros a b H.
+    destruct (classic (a = 0)).
+    - subst.
+      replace (0*b) with 0 in H by ring.
+      now contradiction (one_ne_0_F F).
+    - rewrite <-(inv_r a) in H; auto.
+      assert (a^-1 * (a*b) = a^-1 * (a*a^-1)) as H1 by congruence.
+      now rewrite ? (M2_F F), inv_l, ? (M3_F F) in H1.
+  Qed.
+
+  Theorem inv_one : 1^-1 = 1.
+  Proof.
+    symmetry.
+    apply inv_unique.
+    now rewrite (M3_F F).
+  Qed.
+
+  Theorem inv_neg : ∀ a, a ≠ 0 → -a^-1 = (-a)^-1.
+  Proof.
+    intros a H.
+    field.
+    split; auto.
+    contradict H.
+    ring [H].
+  Qed.
+
+  Theorem inv_ne_0 : ∀ a, a ≠ 0 → a^-1 ≠ 0.
+  Proof.
+    intros a H H0.
+    pose proof (inv_r a H) as H1.
+    rewrite H0 in H1.
+    replace (a*0) with 0 in H1 by ring.
+    now contradiction (one_ne_0_F F).
+  Qed.
+
+  Theorem inv_inv : ∀ a, a ≠ 0 → a^-1^-1 = a.
+  Proof.
+    intros a H.
+    assert (a * a^-1 * a = a * a^-1 * a^-1^-1) as H0.
+    { rewrite <-? M2_F, inv_l,  (M1_F _ (a^-1)), inv_l; auto using inv_ne_0. }
+      now rewrite ? (M1_F _ a), inv_l, ? M3_F in H0.
+  Qed.
 
 End Field_theorems.
